Added load path, proved Reflection and stuff

MyReflection.v
@@ -18,11 +18,6 @@ Proof. split.
   inversion H2.
 Qed.
 
-Theorem lebP : forall n m, reflect (le n m) (leb n m).
-Proof. intros. apply reflect_iff. split.
-- apply leb_correct.
-- apply leb_complete. Qed.
-
 Fixpoint count n l :=
   match l with
   | nil => 0
@@ -39,6 +34,33 @@ Proof. induction l; intros.
     * destruct n0. auto.
     * auto. Qed.
 
+Definition simple_reflect (P: Prop) (b: bool) : Prop :=
+  (P /\ b = true) \/ (~P /\ b = false).
+
+Theorem simple_reflect_iff: forall P b,
+  simple_reflect P b <-> (P <-> b = true).
+Proof. intros. split; intros.
+- inversion H; destruct H0; auto.
+  + split; auto. + split; auto. intro. rewrite H1 in H2; inversion H2.
+- destruct H. unfold simple_reflect. destruct b.
+  + left; auto. + right; auto. split; auto.
+  intro. apply H in H1; inversion H1. Qed.
+
+Theorem simple_beq_natP : forall n m,
+  simple_reflect (n = m) (n =? m).
+Proof. intros. apply simple_reflect_iff.
+symmetry. apply Nat.eqb_eq. Qed.
+
+Theorem simple_beq_natP_practice : forall n l,
+  count n l = 0 -> ~(In n l).
+Proof. induction l; intros.
+- intro. inversion H0.
+- intro. inversion H. destruct (simple_beq_natP n a); destruct H1.
+  + rewrite H3 in H2. inversion H2.
+  + rewrite H3 in H2. inversion H2. 
+  apply IHl in H5. apply H5. inversion H0.
+    * subst. exfalso; apply H1. auto.
+    * auto. Qed.
 
 
 
