Dirichlet.v
@@ -1,0 +1,22 @@
+Require Import List.
+
+Definition Decidable (T: Type):= forall (n m: T),
+  n = m \/ n <> m.
+
+Theorem In_Decidable: forall (T: Type) (l: list T) (n: T),
+   Decidable T ->
+  In n l \/ ~ In n l.
+Proof. induction l; intros.
+- right. auto.
+- assert (In n l \/ ~ In n l).
+{ apply (IHl n). auto. }
+destruct H0.
+  + left. simpl. right. assumption.
+  + simpl. assert (a = n \/ a <> n).
+  { apply (H a n). }
+  destruct H1.
+    * left. left; assumption.
+    * right. intro. destruct H2. apply H1 in H2; auto.
+    apply H0 in H2; auto. Qed.
+
+(*Now we can prove the Dirichlet principle with this result*)
